Tests/Completeness/LayoutCorridor.lean
@@ -3,7 +3,7 @@ Copyright (c) 2026 Bangyen Pham. All rights reserved.
 Released under Apache 2.0 license as described in the file LICENSE.
 Authors: Bangyen Pham
 -/
-import LeanFunge.Theory.Completeness.LayoutCorridor
+import LeanFunge.Theory.Completeness.LayoutRouting
 import LeanFunge.Theory.Completeness.LayoutRouting
 
 /-!
