Tests/Completeness/LayoutSimulation.lean
@@ -3,8 +3,8 @@ Copyright (c) 2026 Bangyen Pham. All rights reserved.
 Released under Apache 2.0 license as described in the file LICENSE.
 Authors: Bangyen Pham
 -/
-import LeanFunge.Theory.Completeness.LayoutSimulationRun
-import LeanFunge.Theory.Completeness.LayoutSimulationUniversal
+import LeanFunge.Theory.Completeness.LayoutSimulation
+import LeanFunge.Theory.Completeness.LayoutSimulationNormalize
 
 /-!
 # Simulation Tests
